Equality fixes.

examples/preorders/MRefHeap.fst
@@ -7,8 +7,8 @@ open Preorder
    (represented as natural numbers) to types, values and preorders. *)
 
 abstract type heap = h:(nat * (nat -> Tot (option (dtuple2 Type0 (fun a -> a * r:relation a{preorder r})))))
-		       {(forall (n:nat) . n < fst h ==> (exists v . snd h n = Some v)) /\ 
-			(forall (n:nat) . n >= fst h ==> snd h n = None)}
+		       {(forall (n:nat) . n < fst h ==> (exists v . snd h n == Some v)) /\ 
+			(forall (n:nat) . n >= fst h ==> snd h n == None)}
 
 (* References. *)
 
@@ -19,9 +19,9 @@ abstract type mref (a:Type) (r:relation a{preorder r}) = nat
 
 let contains (#a:Type) (#r:relation a{preorder r}) (h:heap) (m:mref a r) = 
   exists v . 
-    snd h m = Some v /\ 
-    dfst v = a /\ 
-    snd #a #(r:relation a{preorder r}) (dsnd v) = r
+    snd h m == Some v /\ 
+    dfst v == a /\ 
+    snd #a #(r:relation a{preorder r}) (dsnd v) == r
 
 
 (* Select. *)
@@ -44,15 +44,15 @@ val alloc_ref : h0:heap ->
 	        x:a -> 
 		Tot (mh1:(mref a r * heap){~(contains #a #r h0 (fst mh1)) /\ 
 		                           contains (snd mh1) (fst mh1) /\
-		                           sel (snd mh1) (fst mh1) = x /\
+		                           sel (snd mh1) (fst mh1) == x /\
 					   (forall b r' (m:mref b r') .  
 			                      contains h0 m 
 			                      ==> 
 			                      contains (snd mh1) m) /\
 			                   (forall b r' (m:mref b r'{contains h0 m}) y . 
-			                      sel #b h0 m = y 
+			                      sel #b h0 m == y 
 		                              ==> 
-			                      sel #b (snd mh1) m = y)})
+			                      sel #b (snd mh1) m == y)})
 let alloc_ref h a r x = 
   (fst h , (fst h + 1 , (fun n -> if n = fst h then Some (| a , (x , r) |)
 					       else snd h n)))
@@ -66,15 +66,16 @@ val upd : #a:Type ->
           m:mref a r{contains h0 m} -> 
           x:a -> 
           Tot (h1:heap{contains h1 m /\ 
-	               sel h1 m = x /\
+	               sel h1 m == x /\
 		       (forall b r' (m':mref b r') .  
 			  contains h0 m' 
 			  ==> 
 			  contains h1 m') /\
-		       (forall b r' (m':mref b r'{contains h0 m'}) y . m' =!= m /\ 
-			  sel h0 m' = y 
+		       (forall b r' (m':mref b r'{contains h0 m'}) y . 
+		          ~(m' === m) /\ 
+			  sel h0 m' == y 
 			  ==> 
-			  sel h1 m' = y)})
+			  sel h1 m' == y)})
 let upd #a #r h0 m x = 
   (fst h0 , (fun m' -> if m = m' then Some (| a , (x , r) |)
                                  else snd h0 m'))
